Start improving vector definitions

HOTG/Functors/HOTG_Lists.thy
@@ -1,5 +1,5 @@
 theory HOTG_Lists
-  imports HOTG_Functions_Monotone
+  imports HOTG_Functions_Monotone HOTG_Ordinals_Omega ML_Unification.Unification_Attributes
 begin
 
 axiomatization
@@ -7,18 +7,140 @@ axiomatization
   and cons :: "set \<Rightarrow> set \<Rightarrow> set"
   and list_rec :: "'a \<Rightarrow> (set \<Rightarrow> set \<Rightarrow> 'a \<Rightarrow> 'a) \<Rightarrow> set \<Rightarrow> 'a"
   and list :: "set \<Rightarrow> set \<Rightarrow> bool"
-  where nil_ne_cons[iff]: "nil \<noteq> cons x xs"
-  and cons_inj[iff]: "cons x xs = cons y ys \<longleftrightarrow> (x = y \<and> xs = ys)"
+  where nil_ne_cons[iff]: "\<And>x xs. nil \<noteq> cons x xs"
+  and cons_inj[iff]: "\<And>x xs y ys. cons x xs = cons y ys \<longleftrightarrow> (x = y \<and> xs = ys)"
   and nil_type: "\<And>A. (list A) nil"
   and cons_type: "\<And>A. (mem_of A \<Rightarrow> list A \<Rightarrow> list A) cons"
   and list_rec_nil: "\<And>n c. list_rec n c nil = n"
   and list_rec_cons: "\<And>n c x xs. list_rec n c (cons x xs) = c x xs (list_rec n c xs)"
   and list_rec_type: "\<And>(P :: 'a \<Rightarrow> bool) A. 
     (P \<Rightarrow> (mem_of A \<Rightarrow> list A \<Rightarrow> P \<Rightarrow> P) \<Rightarrow> list A \<Rightarrow> P) list_rec"
-  and list_induct[case_names nil cons, induct type: set, consumes 1]: "\<And>A P. list A xs \<Longrightarrow> P nil \<Longrightarrow>
+  and list_induct[case_names nil cons, induct type: set, consumes 1]: "\<And>A P xs. list A xs \<Longrightarrow> P nil \<Longrightarrow>
     (\<And>x xs. x \<in> A \<Longrightarrow> list A xs \<Longrightarrow> P xs \<Longrightarrow>  P (cons x xs)) \<Longrightarrow> P xs"
 
+unbundle no_HOL_groups_syntax no_HOL_ascii_syntax no_HOL_order_syntax
+
+definition "length \<equiv> list_rec 0 (\<lambda>_ _. succ)"
+
+lemma length_nil_eq[simp]: "length nil = 0"
+  unfolding length_def by (fact list_rec_nil)
+
+lemma length_cons_eq_succ[simp]: "length (cons x xs) = succ (length xs)"
+  unfolding length_def using list_rec_cons[of _ "\<lambda>_ _. succ"] by simp
+
+lemma length_type: "(list A \<Rightarrow> mem_of \<omega>) length"
+proof-
+  have T1: "(mem_of A \<Rightarrow> list A \<Rightarrow> mem_of \<omega> \<Rightarrow> mem_of \<omega>) (\<lambda> _ _ . succ)" 
+    using succ_mem_omega_if_mem by blast
+  have T2: "mem_of \<omega> 0" by auto
+  from list_rec_type[THEN mono_wrt_predD, THEN mono_wrt_predD, OF T2 T1]
+  show ?thesis using list_rec_type unfolding length_def by blast
+qed
+
+definition "is_nil = list_rec True (\<lambda>_ _ _. False)"
+
+lemma "is_nil nil"
+  unfolding is_nil_def using list_rec_nil[of True] by blast
+
+lemma "\<And>x xs. \<not>is_nil (cons x xs)"
+  unfolding is_nil_def using list_rec_cons[of True "(\<lambda>_ _ _. False)"] by blast
+
+definition "is_cons = list_rec False (\<lambda>_ _ _. True)"
+
+definition "head = list_rec undefined (\<lambda>x _ _. x)"
+
+lemma head_type: "(list A \<Rightarrow> mem_of A) head"
+proof-
+  have "(mem_of A \<Rightarrow> list A \<Rightarrow> mem_of A \<Rightarrow> mem_of A) (\<lambda>x _ _. x)" by blast
+  with list_rec_type[where ?P="list A"] show ?thesis unfolding head_def sorry (*needs: mem_of A undefined*)
+qed
+
+definition "tail = list_rec undefined (\<lambda>_ xs _. xs)"
+
+lemma tail_type: "(list A \<Rightarrow> list A) tail"
+proof-
+  have "(mem_of A \<Rightarrow> list A \<Rightarrow> list A \<Rightarrow> list A) (\<lambda>_ xs _. xs)" by blast
+  with list_rec_type[where ?P="list A"] show ?thesis unfolding tail_def sorry (*needs: list A undefined*)
+qed
+
+
+definition "map f \<equiv> list_rec nil (\<lambda>x _. cons (f x))"
+
+lemma map_type: 
+  assumes "(mem_of A \<Rightarrow> mem_of B) f"
+  shows "(list A \<Rightarrow> list B) (map f)"
+proof -
+  have "(mem_of A \<Rightarrow> list A \<Rightarrow> list B \<Rightarrow> list B) (\<lambda>x _. cons (f x))"
+    using cons_type assms by blast
+  with list_rec_type[where ?P="list B"] nil_type show ?thesis unfolding map_def by blast
+qed
+
+lemma map_nil_eq[simp]: "map f nil = nil"
+  by (simp add: map_def list_rec_nil)
+
+lemma map_cons_eq[simp]: "map f (cons x xs) = cons (f x) (map f xs)"
+  by (simp add: map_def list_rec_cons)
+
+definition "index_list \<equiv> list_rec nil (\<lambda>x _ xs. cons \<langle>0,x\<rangle> (map (\<lambda>p. \<langle>succ (fst p), snd p\<rangle>) xs))"
+
+lemma index_list_type: "(list A \<Rightarrow> list (\<omega> \<times> A)) index_list"
+proof-
+  have "(mem_of (\<omega> \<times> A) \<Rightarrow> mem_of (\<omega> \<times> A)) (\<lambda>p. \<langle>succ (fst p), snd p\<rangle>)" by auto
+  then have "(list (\<omega> \<times> A) \<Rightarrow> list (\<omega> \<times> A)) (map (\<lambda>p. \<langle>succ (fst p), snd p\<rangle>))" using map_type by auto
+  then have "(mem_of A \<Rightarrow> list A \<Rightarrow> list (\<omega> \<times> A) \<Rightarrow> list (\<omega> \<times> A)) (\<lambda>x _ xs. cons \<langle>0,x\<rangle> (map (\<lambda>p. \<langle>succ (fst p), snd p\<rangle>) xs))" using cons_type[of "\<omega> \<times> A"] by fastforce
+  with list_rec_type[where ?P="list (\<omega> \<times> A)"] nil_type show ?thesis unfolding index_list_def by auto
+qed
+
+definition "nth n xs \<equiv> list_rec undefined (\<lambda>x _ res. (if (fst x = n) then snd x else res)) (index_list xs)"
+
+lemma nth_type: "(mem_of \<omega> \<Rightarrow> list A \<Rightarrow> mem_of A) nth"
+  sorry
+
+
+definition "tuple Ps xs \<equiv> length Ps = length xs \<and> (\<forall>i. 0 \<le> i \<and> i < (length xs) \<longrightarrow> mem_of (nth i Ps) (nth i xs))"
+
+lemma tuple_nil[simp]: "tuple nil nil" 
+  unfolding tuple_def by auto
+
+lemma tuple_cons: "x \<in> p \<Longrightarrow> tuple Ps xs \<Longrightarrow> tuple (cons p Ps) (cons x xs)" 
+  sorry
+
+definition "replicate n x \<equiv> omega_rec nil (cons x) n"
+
+lemma replicate_zero[simp]: "\<And>x. replicate 0 x = nil" unfolding replicate_def by auto
+
+lemma replicate_type: "(mem_of \<omega> \<Rightarrow> mem_of A \<Rightarrow> list A) replicate"
+  sorry
+
+lemma replicate_succ: "n \<in> \<omega> \<Longrightarrow> replicate (succ n) x = cons x (replicate n x)"
+  unfolding replicate_def by (rule omega_rec_succ)
+
+lemma replicate_nth: " \<forall>i. 0 \<le> i \<and> i < n \<longrightarrow> nth i (replicate n x) = x"
+  sorry
+
+lemma "list P xs = tuple (replicate (length xs) P) xs"
+proof
+  assume "list P xs"
+  then show "tuple (replicate (length xs) P) xs" proof (induction xs rule: list_induct)
+    case nil
+    then show ?case unfolding tuple_def by auto
+  next
+    case (cons x xs)
+    then have "replicate (length (cons x xs)) P = cons P (replicate (length xs) P)" using replicate_succ length_type by auto
+    then show ?case using tuple_cons cons by auto
+  qed
+next 
+  assume "tuple (replicate (length xs) P) xs"
+  then have "\<forall> i. 0 \<le> i \<and> i < length xs \<longrightarrow> mem_of P (nth i xs)" using replicate_nth tuple_def by auto
+  then show "list P xs" sorry
+qed
+
+definition "vector P n xs \<equiv> length xs = n \<and> list P xs"
+
 definition "append xs ys \<equiv> list_rec ys (\<lambda>x _. cons x) xs"
+
+lemma "list A (cons x xs) \<Longrightarrow> mem_of A x \<and> list A xs"
+ by (induction "(cons x xs)" rule: list_induct) auto
 
 lemma nil_append_eq [simp]: "append nil ys = ys"
   by (simp add: list_rec_nil append_def)
@@ -54,23 +176,6 @@ proof -
   with list_rec_type[where ?P="list A"] nil_type show ?thesis unfolding rev_def 
     by blast
 qed
-
-definition "map f \<equiv> list_rec nil (\<lambda>x _. cons (f x))"
-
-lemma map_type: 
-  assumes "(mem_of A \<Rightarrow> mem_of B) f"
-  shows "(list A \<Rightarrow> list B) (map f)"
-proof -
-  have "(mem_of A \<Rightarrow> list A \<Rightarrow> list B \<Rightarrow> list B) (\<lambda>x _. cons (f x))"
-    using cons_type assms by blast
-  with list_rec_type[where ?P="list B"] nil_type show ?thesis unfolding map_def by blast
-qed
-
-lemma map_nil_eq[simp]: "map f nil = nil"
-  by (simp add: map_def list_rec_nil)
-
-lemma map_cons_eq[simp]: "map f (cons x xs) = cons (f x) (map f xs)"
-  by (simp add: map_def list_rec_cons)
 
 
 end
