HOTG/Functors/HOTG_Vectors.thy
@@ -2,26 +2,7 @@ theory HOTG_Vectors
   imports HOTG_Lists HOTG_Ordinals_Omega ML_Unification.Unification_Attributes
 begin
 
-unbundle no_HOL_groups_syntax
 
-definition "length \<equiv> list_rec 0 (\<lambda>_ _. succ)"
-
-lemma length_nil_eq[simp]: "length nil = 0"
-  unfolding length_def by (fact list_rec_nil)
-
-lemma length_cons_eq_succ[simp]: "length (cons x xs) = succ (length xs)"
-  unfolding length_def using list_rec_cons[of _ "\<lambda>_ _. succ"] by simp
-
-lemma length_type: "(list A \<Rightarrow> mem_of \<omega>) length"
-proof-
-  have T1: "(mem_of A \<Rightarrow> list A \<Rightarrow> mem_of \<omega> \<Rightarrow> mem_of \<omega>) (\<lambda> _ _ . succ)" 
-    using succ_mem_omega_if_mem by blast
-  have T2: "mem_of \<omega> 0" by auto
-  from list_rec_type[THEN mono_wrt_predD, THEN mono_wrt_predD, OF T2 T1]
-    show ?thesis using list_rec_type unfolding length_def by blast
-qed
-
-definition "vector A n xs \<equiv> list A xs \<and> length xs = n"
 
 
 axiomatization 
@@ -41,6 +22,6 @@ axiomatization
 
 definition "fun_vector_compose \<equiv> vector_rec_2 nil (\<lambda> (f::set) (g::set) _ _ zs . cons (g \<circ>\<circ> f) zs)"
 
-
+(* todo: zipwith *)
 
 end
